Java/src/Logic/AssertionLogic.v
@@ -1,14 +1,15 @@
+(* This file is a monster. Working with type classes is great, but the mechanisms for
+   creating an instance are currently very fragile. One major piece of work will be to
+   make this easier. Ideally, this file should not be larger than a few tens of lines
+   at most. *)
+
 Require Import ILogic ILInsts SepAlg SepAlgPfun BILogic BILInsts IBILogic SepAlgMap Maps String Rel.
 Require Import RelationClasses Setoid Morphisms Program. 
 Require Import MapInterface MapFacts.
-Require Import Open Stack Lang Pure ILEmbed.
+Require Import Open Stack Lang OpenILogic Pure ILEmbed.
 
 Local Existing Instance ILPre_Ops.
 Local Existing Instance ILPre_ILogic.
-(*
-Local Existing Instance ILPartial_Ops.
-Local Existing Instance ILPartial_Logic.
-*)
 
 Local Existing Instance ILFun_Ops.
 Local Existing Instance ILFun_ILogic.
@@ -19,10 +20,6 @@ Local Existing Instance IBILPreLogic.
 Local Existing Instance BILFun_Ops.
 Local Existing Instance IBILFunLogic.
 
-(*
-Local Existing Instance BILPartial_Ops.
-Local Existing Instance BILPartialLogic.
-*)
 Local Existing Instance MapSepAlgOps.
 Local Existing Instance MapSepAlg.
 Local Existing Instance MapEquiv.
@@ -38,24 +35,84 @@ Instance HeapSepAlgOps : SepAlgOps heap := _.
 Instance SepAlgHeap : SepAlg heap := _.
 
 Definition asn1 := ILPreFrm (@rel heap subheap) Prop.
-Definition asn2 := ILPreFrm ge asn1.
-Definition asn := ILPreFrm Prog_wf_sub asn2.
-
 Instance ILogicOpsAsn1 : ILogicOps asn1 := _.
-Instance ILogicOpsAsn2 : ILogicOps asn2 := _.
-Instance ILogicOpsAsn : ILogicOps asn := _.
-
 Instance ILogicAsn1 : ILogic asn1 := _.
+
+
+Definition asn2 := ILPreFrm ge asn1.
+Instance ILogicOpsAsn2 : ILogicOps asn2 := _.
 Instance ILogicAsn2 : ILogic asn2 := _.
+
+Definition asn := ILPreFrm Prog_wf_sub asn2.
+Instance ILogicOpsAsn : ILogicOps asn := _.
 Instance ILogicAsn : ILogic asn := _.
 
 Instance BILOperatorsAsn1 : BILOperators asn1 := _.
 Instance BILOperatorsAsn2 : BILOperators asn2 := _.
 Instance BILOperatorsAsn : BILOperators asn := _.
 
+Instance BILogicAsn1 : BILogic asn1 := _.
+Instance BILogicAsn2 : BILogic asn2 := _.
+Instance BILogicAsn  : BILogic asn := _.
+
 Instance IBILogicAsn1 : IBILogic asn1 := _.
 Instance IBILogicAsn2 : IBILogic asn2 := _.
 Instance IBILogicAsn  : IBILogic asn := _.
+
+Local Existing Instance EmbedILPreDropOpEq.
+Local Existing Instance EmbedILPreDropEq.
+Local Existing Instance EmbedILPreDropOpNeq.
+Local Existing Instance EmbedILPreDropNeq.
+
+Instance EmbedAsnPropOp : EmbedOp Prop asn := _.
+Instance EmbedAsnProp : Embed Prop asn := _.
+
+Definition sasn := @open var _ asn.
+
+Instance ILOpsSAsn : ILogicOps sasn := _.
+Instance ILogicSAsn : ILogic sasn := _.
+Instance BILOperatorsSAsn : BILOperators sasn := _.
+Instance BILogicSAsn : IBILogic sasn := _.
+
+Local Existing Instance EmbedILFunDropOp.
+Local Existing Instance EmbedILFunDrop.
+Local Existing Instance EmbedILPreDropOpEq.
+Local Existing Instance EmbedILPreDropEq.
+Local Existing Instance EmbedILPreDropOpNeq.
+Local Existing Instance EmbedILPreDropNeq.
+Local Existing Instance EmbedILFunOp.
+Local Existing Instance EmbedILFun.
+Local Existing Instance EmbedILPreOp.
+Local Existing Instance EmbedILPre.
+
+Local Existing Instance EmbedPropPure.
+Local Existing Instance PureFunDrop.
+Local Existing Instance PureFun.
+Local Existing Instance PurePreDrop.
+Local Existing Instance PurePre.
+ 
+Instance PurePure (P : pure) : @Pure sasn _ _ (embed P) := _.
+
+Instance EmbedSasnPureOp : EmbedOp pure sasn := _.
+Instance EmbedSasnPure : Embed pure sasn := _.
+
+Require Import SpecLogic.
+
+Instance EmbedAsn1PropOp : EmbedOp Prop asn1 := _.
+Instance EmbedAsn1Prop   : Embed Prop asn1 := _.
+Instance EmbedAsn2SpecOp : EmbedOp spec1 asn2 := _.
+Instance EmbedAsn2Spec   : Embed spec1 asn2 := _.
+Instance EmbedAsnSpecOp  : EmbedOp spec asn := _.
+Instance EmbedAsnSpec    : Embed spec asn := _.
+Instance EmbedSAsnSpecOp : EmbedOp spec sasn := _.
+Instance EmbedSAsnSpec   : Embed spec sasn := _.
+
+Instance PureProp (P : Prop) : @Pure asn1 ILogicOpsAsn1 BILOperatorsAsn1 (embed P) := _.
+Instance PureSpec1 (S : spec1) : @Pure asn2 ILogicOpsAsn2 BILOperatorsAsn2 (embed S) := _.
+Instance PureSpecAsn (S : spec) : @Pure asn _ _ (embed S) := _.
+Instance PureSpec (S : spec) : @Pure sasn _ _ (embed S) := _.
+
+
 Local Transparent ILPre_Ops.
 
 Definition mk_asn (f: Prog_wf -> nat -> heap -> Prop)
@@ -81,42 +138,5 @@ Next Obligation.
   setoid_rewrite H in H0. assumption.
 Qed.
 
-
-Local Existing Instance EmbedILPreDropOpEq.
-Local Existing Instance EmbedILPreDropEq.
-Local Existing Instance EmbedILPreDropOpNeq.
-Local Existing Instance EmbedILPreDropNeq.
-
-Instance EmbedAsnPropOp : EmbedOp Prop asn := _.
-Instance EmbedAsnProp : Embed Prop asn := _.
-
 Program Definition pointsto (p : val) (f : field) (v : val) : asn :=
   (p <> null) /\\ pointsto_aux (val_to_ptr p) f v.
-
-Definition sasn := @open var _ asn.
-
-Instance ILOpsSAsn : ILogicOps sasn := _.
-Instance ILogicSAsn : ILogic sasn := _.
-Instance BILOperatorsSAsn : BILOperators sasn := _.
-Instance BILogicSAsn : IBILogic sasn := _.
-
-Local Existing Instance EmbedILFunDropOp.
-Local Existing Instance EmbedILFunDrop.
-Local Existing Instance EmbedILPreDropOpEq.
-Local Existing Instance EmbedILPreDropEq.
-Local Existing Instance EmbedILPreDropOpNeq.
-Local Existing Instance EmbedILPreDropNeq.
-Local Existing Instance EmbedILFunOp.
-Local Existing Instance EmbedILFun.
-Local Existing Instance EmbedILPreOp.
-Local Existing Instance EmbedILPre.
-
-Instance EmbedAsnPureOp : EmbedOp pure sasn := _.
-Instance EmbedAsnPure : Embed pure sasn := _.
-
-Require Import SpecLogic.
-
-Instance EmbedAsnSpecOp : EmbedOp spec sasn := _.
-Instance EmbedAsnSpec : Embed spec sasn := _.
-
-
