Java/src/Semantics/SemCmd.v
@@ -1,4 +1,4 @@
-Require Import Program SepAlg Pure AssertionLogic SpecLogic SepAlgMap.
+Require Import Program SepAlg OpenILogic AssertionLogic SpecLogic SepAlgMap.
 Require Import MapInterface MapFacts.
 Require Import ILInsts ILogic ILEmbed Open Subst Stack Lang.
 
