Java/src/Semantics/SemCmdRules.v
@@ -1,5 +1,5 @@
 Require Import SemCmd ILogic BILogic ILInsts BILInsts. 
-Require Import Pure Later AssertionLogic SpecLogic ILEmbed.
+Require Import OpenILogic Later AssertionLogic SpecLogic ILEmbed.
 Require Import Stack Subst Lang Util List.
 Require Import FunctionalExtensionality.
 
